Extract option types as pairs
This is easier than adding pointers to the semantics, since we already
have pairs working. The idea is that for an option T, the pair is of
type bool * T, where the first element is true iff the second is valid.

src/Facade.v
@@ -114,6 +114,15 @@ Proof.
             wrap_type := Go.Slice wrap_type |}; GoWrapper_t.
 Defined.
 
+Instance GoWrapper_option {A} {WA : GoWrapper A} : GoWrapper (option A).
+Proof.
+  refine {| wrap' := fun o => match o with
+                              | None => (false, Go.moved_value' _ (Go.default_value' _))
+                              | Some x => (true, wrap' x) end;
+            wrap_type := Go.Pair Go.Bool (@wrap_type _ WA)|}.
+  intros a b H.
+  destruct a, b; invc H; GoWrapper_t.
+Defined.
 
 Instance GoWrapper_dec {P Q} : GoWrapper ({P} + {Q}).
 Proof.
@@ -861,7 +870,9 @@ Ltac pred_solve_step := match goal with
   end.
 
 Ltac pred_solve := progress (
-  repeat (unfold pred_apply in *; rewrite ?add_upd, ?remove_delete, ?default_zero);
+  unfold pred_apply in *;
+  repeat pred_solve_step;
+  repeat rewrite ?add_upd, ?remove_delete, ?default_zero;
   repeat pred_solve_step).
 
 Lemma Declare_fail :
@@ -2120,6 +2131,127 @@ Proof.
 Qed.
 
 Hint Constructors source_stmt.
+
+Definition option2pair {T} {H : GoWrapper T} {D : DefaultValue T} (o : option T) : bool * T :=
+  match o with
+  | None => (false, zeroval)
+  | Some t => (true, t)
+  end.
+
+Lemma CompileRetOptionSome : forall env B {HB: GoWrapper B} {D : DefaultValue B}
+  avar bvar pvar (b : B) (p : bool * B) F,
+  EXTRACT Ret (Some b)
+  {{ avar ~> true * bvar ~> b * pvar ~> p * F }}
+    Modify JoinPair (pvar, avar, bvar)
+  {{ fun ret => pvar ~> option2pair ret *
+                avar |-> moved_value (wrap true) *
+                bvar |-> moved_value (wrap b) * F }} // env.
+Proof.
+  intros.
+  unfold ProgOk.
+  inv_exec_progok.
+  - repeat inv_exec.
+    repeat econstructor.
+    eval_expr.
+    pred_solve.
+  - inv_exec_progok.
+  - inv_exec_progok.
+    contradiction H1.
+    repeat econstructor;
+    [ eval_expr; eauto..].
+Qed.
+
+Lemma CompileRetOptionNone : forall env B {HB: GoWrapper B} {D : DefaultValue B}
+  avar pvar (p : bool * B) F,
+  EXTRACT Ret None
+  {{ avar ~> false * pvar ~> p * F }}
+    Declare wrap_type (fun bvar =>
+      Modify JoinPair (pvar, avar, bvar)
+    )
+  {{ fun ret => pvar ~> (option2pair ret) *
+                avar |-> moved_value (wrap false) * F }} // env.
+Proof.
+  intros.
+  eapply CompileDeclare. intro bvar.
+  unfold ProgOk.
+  inv_exec_progok.
+  - repeat inv_exec.
+    repeat econstructor.
+    eval_expr.
+    pred_solve.
+  - inv_exec_progok.
+  - inv_exec_progok.
+    contradiction H1.
+    repeat econstructor;
+    [ eval_expr; eauto..].
+Qed.
+
+Lemma CompileMatchOption : forall env B {HB : GoWrapper B} X {HX : GoWrapper X} {D : DefaultValue B}
+  ovar avar bvar (o : option B) (a0 : bool) (b0 : B) C (F : pred)
+  (pnone : prog X) xpnone (psome : B -> prog X) xpsome,
+  (forall (b : B),
+  EXTRACT (psome b)
+  {{ avar ~> true * bvar ~> b * ovar |-> moved_value (wrap o) * F }}
+    xpsome
+  {{ fun ret => C ret * avar |->? * bvar |->? * ovar |-> moved_value (wrap o)}} // env) ->
+  EXTRACT pnone
+  {{ avar ~> false * bvar ~> zeroval * ovar |-> moved_value (wrap o) * F }}
+    xpnone
+  {{ fun ret => C ret * avar |->? * bvar |->? * ovar |-> moved_value (wrap o) }} // env ->
+  EXTRACT (match o with
+           | None => pnone
+           | Some b => psome b
+           end)
+  {{ ovar ~> (option2pair o) * avar ~> a0 * bvar ~> b0 * F }}
+    Modify SplitPair (ovar, avar, bvar) ;
+    If Var avar Then xpsome Else xpnone EndIf
+  {{ fun ret => C ret * avar |->? * bvar |->? * ovar |-> moved_value (wrap o) }} // env.
+Proof.
+  intros.
+  eapply extract_equiv_prog with (pr1 := Bind (Ret tt) (fun _ => _)).
+  rewrite bind_left_id. apply prog_equiv_equivalence.
+  eapply CompileSeq.
+  eapply hoare_strengthen_pre;
+    [ | apply CompileSplit with (p := option2pair o)].
+  cancel_subset.
+  destruct o; simpl in *.
+  + unfold ProgOk; inv_exec_progok.
+    - inv_exec.
+      inv_exec; eval_expr.
+      edestruct H; eauto.
+      simpl. pred_solve.
+      forward_solve.
+    - inv_exec; inv_exec; eval_expr.
+      edestruct H; eauto.
+      simpl. pred_solve.
+      forward_solve.
+    - inv_exec.
+      inv_exec; eval_expr.
+      edestruct H; eauto.
+      simpl. pred_solve.
+      forward_solve.
+      contradiction H3.
+      repeat eexists. apply StepIfTrue. eval_expr.
+  + repeat rewrite moved_value'_idem in *.
+    erewrite <- default_zero' in * by apply default_zero.
+    unfold ProgOk; inv_exec_progok.
+    - inv_exec.
+      inv_exec; eval_expr.
+      edestruct H0; eauto.
+      simpl. pred_solve.
+      forward_solve.
+    - inv_exec; inv_exec; eval_expr.
+      edestruct H0; eauto.
+      simpl. pred_solve.
+      forward_solve.
+    - inv_exec.
+      inv_exec; eval_expr.
+      edestruct H0; eauto.
+      simpl. pred_solve.
+      forward_solve.
+      contradiction H3.
+      repeat eexists. apply StepIfFalse. eval_expr.
+Qed.
 
 Local Open Scope pred.
 
